theories/clang/notations.v
@@ -38,9 +38,7 @@ Notation "'while' [ c ] ( e ) <{ s }>" := (Ewhile c%E e%E s%E)
   (at level 200, c, e, s at level 200) : expr_scope.
 Notation "s1 ;; s2" := (Eseq s1%E s2%E)
   (at level 100, s2 at level 200, format "s1  ;;  s2") : expr_scope.
-(* Notation "'ret'" := Eret (at level 80): expr_scope. *)
 Notation "'rete' e" := (Erete e%E) (at level 80): expr_scope.
-(* Notation "'skip'" := (Eskip) (at level 200) : expr_scope. *)
 
 Notation "'cli'" := (Eprim Pcli) (at level 80) : expr_scope.
 Notation "'sti'" := (Eprim Psti) (at level 80) : expr_scope.
